Relax level relation between terms and types.
The level of a term merely needs to be less than or equal
to the level of their types.
Coq proofs have been repaired with these new rules.
Removing arrow types entirely remains to be done,
as well as fixing the implementation and the model.

coq/typesafety.v
@@ -4,7 +4,6 @@ Require Export StraTT.basics.
 Require Export StraTT.ctx.
 Require Export StraTT.subst.
 Require Export StraTT.inversion.
-Require Export StraTT.restrict.
 
 Set Implicit Arguments.
 
@@ -16,12 +15,13 @@ Local Open Scope lc_scope.
 
 Inductive Ctx_DEquiv S : context -> context -> Prop :=
  | ctx_equiv_nil : Ctx_DEquiv S nil nil
- | ctx_equiv_cons : forall x i A1 A2 G1 G2,
+ | ctx_equiv_cons : forall x j k A1 A2 G1 G2,
+     j <= k ->
      DEquiv S A1 A2 ->
      Ctx_DEquiv S G1 G2 ->
-     DTyping S G2 A2 a_Type i ->
+     DTyping S G2 A2 a_Type k ->
      x `notin` dom G1 \u dom G2 ->
-     Ctx_DEquiv S (x ~ (Tm A1 i) ++ G1) (x ~ Tm A2 i ++ G2).
+     Ctx_DEquiv S (x ~ (Tm A1 j) ++ G1) (x ~ Tm A2 j ++ G2).
 
 #[global] Hint Constructors Ctx_DEquiv : core.
 
@@ -30,8 +30,8 @@ Lemma binds_Ctx_DEquiv : forall S G1 G2,
     exists A2, binds x (Tm A2 i) G2 /\ DEquiv S A1 A2.
 Proof.
   induction 1; intros; eauto. inversion H.
-  edestruct (binds_cons_1 _ _ _ _ _ _ H3); eauto; split_hyp.
-  - subst. inversion H5. subst.
+  edestruct (binds_cons_1 _ _ _ _ _ _ H4); eauto; split_hyp.
+  - subst. inversion H6. subst.
     exists A2. split; eauto.
   - edestruct IHCtx_DEquiv; eauto. split_hyp.
     exists x1. split; eauto.
@@ -51,7 +51,7 @@ Lemma DCtx_DTyping_conversion :
     DCtx S G1 ->
     forall G2, Ctx_DEquiv S G1 G2 -> DCtx S G2 /\
     forall x A j, binds x (Tm A j) G1
-           -> DTyping S G2 A a_Type j) /\
+           -> exists k, j <= k /\ DTyping S G2 A a_Type k) /\
   (forall S G1 a A k,
     DTyping S G1 a A k ->
     forall G2, Ctx_DEquiv S G1 G2 -> DTyping S G2 a A k).
@@ -66,10 +66,13 @@ Proof.
     specialize (H _ ltac:(eauto)). split_hyp.
     destruct (binds_cons_1 _ _ _ _ _ _ H1).
     + split_hyp. inversion H4. subst.
+      exists k; split. lia.
       eapply DTyping_weakening1.
       eauto.
       econstructor; eauto.
-    + eapply DTyping_weakening1.
+    + destruct (H2 _ _ _ H3) as [k1 [j0k1 HA0]].
+      exists k1; split. lia.
+      eapply DTyping_weakening1.
       eauto.
       econstructor; eauto.
   - specialize (H _ H0).
@@ -82,18 +85,23 @@ Proof.
     move: H => [h0 bb].
     move: (binds_Ctx_DEquiv ltac:(eauto) _ _ _ b)=> b1; eauto.
     destruct b1 as [A2 [b2 Eq]].
-    apply bb in b.
+    destruct (bb _ _ _ b) as [k0 [jk0 HA]].
+    apply DTyping_cumul with (j := j). lia.
     eapply DT_Conv with (A := A2); eauto.
-    apply DTyping_cumul with (j := j); auto.
   - pick fresh x and apply DT_Pi; eauto.
     spec x.
-    eapply H0. eauto with lc.
+    eapply H0.
+    eapply ctx_equiv_cons with (k := k); eauto with lc. lia.
   - pick fresh x and apply DT_AbsTm; eauto.
     spec x.
     eapply H1. eauto with lc.
-  - pick fresh x and apply DT_AbsTy; eauto.
-    spec x.
-    eapply H0. eauto with lc.
+  - pick fresh x and apply DT_AbsTy; spec x; eauto.
+    + eapply H0.
+      eapply ctx_equiv_cons with (k := k); eauto. lia.
+      eauto with lc.
+    + eapply H1.
+      eapply ctx_equiv_cons with (k := k); eauto. lia.
+      eauto with lc.
   - specialize (H _ H0).
     move: H => [h0 _].
     eauto.
@@ -109,6 +117,7 @@ Proof.
   eapply DCtx_DTyping_conversion; eauto.
 Qed.
 
+(*
 Lemma SubG_float_restrict :
     forall G j k, j <= k -> SubG G (float j k (restrict G j)).
 Proof.
@@ -120,8 +129,9 @@ Proof.
   econstructor; eauto.
   econstructor; eauto.
 Qed.
+*)
 
-#[local] Hint Resolve SubG_float_restrict Ctx_DEquiv_refl : core.
+#[local] Hint Resolve (* SubG_float_restrict *) Ctx_DEquiv_refl : core.
 
 Lemma Reduce_Preservation : forall S G a b,
     Reduce S a b
@@ -129,8 +139,8 @@ Lemma Reduce_Preservation : forall S G a b,
 Proof.
   induction 1; intros B k0 DT.
   - (* beta *)
-    move: (DTyping_a_App_inversion DT) => [ARR|PI].
-    -- (* arrow *)
+    move: (DTyping_a_App_inversion DT) => PI.
+    (* -- (* arrow *)
       move: ARR => [A [DABS Da]].
       pick fresh x.
       move: (DTyping_regularity DABS) => h.
@@ -160,63 +170,56 @@ Proof.
          eapply DCtx_cumul; eauto.
       ++ move: Y => [A3 Z]. split_hyp. subst.
          (* impossible. by consistency of DEquiv *)
-         eapply ineq_Arrow_Pi in H3. contradiction.
+         eapply ineq_Arrow_Pi in H3. contradiction. *)
     -- (* pi *)
       move: PI => [j [A0 [B0 [TABS [Ta EQ]]]]].
-      move: (DTyping_regularity TABS) => h.
+      move: (DTyping_regularity TABS) => [k [k0k h]].
       pick fresh x.
       eapply (@DTyping_a_Pi_inversion x) in h. split_hyp.
       eapply (@DTyping_a_Abs_inversion x) in TABS; eauto.
-      move: TABS => [j1 [j2 [A1 [A2 [h [X | Y]]]]]]. split_hyp.
-      ++ (* impossible. by consistency of DEquiv *)
-        apply DE_Sym in H4.
-        eapply ineq_Arrow_Pi in H4. contradiction.
-      ++ move: Y => [A3 Z]. split_hyp. subst.
+      move: TABS => [j1 [A1 [A2 [h [A3 Z]]]]]. split_hyp.
       (* Consistency of DEquiv *)
       have E1: (DEquiv S A1 A0).  eapply DEquiv_Pi_inj1; eauto.
       have E2: (DEquiv S (open B0 a) (open A3 a)).
                eapply DEquiv_Pi_inj3; eauto with lc.
       have E3: (j = j1). eapply DEquiv_Pi_inj2; eauto.
       subst.
-      eapply DT_Conv with (A:= open A3 a); auto.
+      apply DTyping_regularity in DT as [k1 [k0k1 TB]].
+      eapply DT_Conv with (A := open A3 a) (k := k1); auto.
       rewrite (subst_tm_intro x b); auto.
       rewrite (subst_tm_intro x A3); auto.
       simpl_env in h.
       eapply DTyping_subst1; eauto.
       eapply DTyping_cumul; eauto.
       eapply DCtx_conversion; eauto with ctx.
-      eapply DTyping_regularity; eauto.
+      eapply ctx_equiv_cons with (k := k); eauto with ctx. lia.
       eapply DE_Sym. eapply DE_Trans; eauto.
       ++ auto.
-  - have DS: DSig S. eauto with ctx.
+  - (* delta *)
+    have DS: DSig S. eauto with ctx.
     move: (DTyping_a_Const_inversion DT) => [a0 [A0 [j h]]].
     split_hyp.
     have U :uniq S. eauto using DSig_uniq.
-    eapply DT_Conv with (A := (incr i A0)); auto.
-    2: { eapply DTyping_regularity; eauto. }
+    apply DTyping_regularity in DT as [k1 [k0k1 TB]].
+    eapply DT_Conv with (A := incr i A0) (k := k1); auto.
     replace G with (G ++ nil). 2: simpl_env; auto.
     eapply DTyping_weakening1 with (E:=nil)(F:=G).
     2: {  simpl_env; eauto with ctx. }
-
     move: (binds_unique _ _ _ _ _ H H1 U) => u. inversion u. subst.
-    apply DSig_regularity in H1; auto. split_hyp.
+    apply DSig_regularity in H1 as [k [jk [Ta0 TA0]]]; auto.
     replace nil with (IncG i nil). 2: { auto. }
     apply DTyping_cumul with (j := i + j); auto. lia.
     eapply DTyping_incr; eauto.
   - (* app cong *)
-    move: (DTyping_a_App_inversion DT) => [ARR|PI].
-    ++ move: ARR => [A [Tb Ta]].
+    move: (DTyping_a_App_inversion DT) => PI.
+    (* ++ move: ARR => [A [Tb Ta]].
        apply IHReduce in Tb.
-       eapply DT_AppTm; eauto.
+       eapply DT_AppTm; eauto. *)
     ++ move: PI => [j [A0 [B0 [Tb [Ta E]]]]].
        apply IHReduce in Tb.
-       eapply DT_Conv with (A:= open B0 a).
+       apply DTyping_regularity in DT as [k [k0k TB]].
+       eapply DT_Conv with (A := open B0 a) (k := k); auto.
        eapply DT_AppTy; eauto.
-       pick fresh x.
-       move: (DTyping_regularity Tb) => TPi.
-       move: (@DTyping_a_Pi_inversion x _ _ _ _ _ _ TPi ltac:(auto)) => h. split_hyp. auto.
-       eapply DTyping_regularity; eauto.
-       eapply DE_Sym; auto.
 Qed.
 
 Lemma WHNF_Preservation : forall S a b, WHNF S a b ->
