coq/inversion.v
@@ -3,7 +3,6 @@ Require Export StraTT.tactics.
 Require Export StraTT.basics.
 Require Export StraTT.ctx.
 Require Export StraTT.subst.
-Require Export StraTT.restrict.
 
 Set Implicit Arguments.
 
@@ -13,7 +12,7 @@ Local Open Scope lc_scope.
 Lemma DTyping_a_Pi_inversion1 : forall x S G j A B C k,
     DTyping S G (a_Pi A j B) C k ->
     x `notin` dom G \u dom S ->
-    DEquiv S C a_Type /\ DTyping S G A a_Type j /\
+    DEquiv S C a_Type /\ DTyping S G A a_Type k /\
     j < k /\ DTyping S (x ~ Tm A j ++ G) (open_tm_wrt_tm B (a_Var_f x)) a_Type k.
 Proof.
   intros. dependent induction H.
@@ -48,7 +47,7 @@ Qed.
 Lemma DTyping_a_Pi_inversion : forall x S G j A B k,
     DTyping S G (a_Pi A j B) a_Type k ->
     x `notin` dom G \u dom S ->
-    DTyping S G A a_Type j /\
+    DTyping S G A a_Type k /\
     j < k /\ DTyping S (x ~ Tm A j ++ G) (open_tm_wrt_tm B (a_Var_f x)) a_Type k.
 Proof.
   intros.
@@ -75,142 +74,109 @@ Qed.
 
 (* --------------- regularity ----------------- *)
 
-Lemma DTyping_regularity : (forall S G a A k, DTyping S G a A k -> DTyping S G A a_Type k).
+Lemma DTyping_regularity : (forall S G a A j, DTyping S G a A j -> exists k, j <= k /\ DTyping S G A a_Type k).
 Proof.
   induction 1; eauto.
   - (* const *)
     have DS: DSig S. eapply DCtx_DSig; eauto.
-    eapply DSig_regularity in H; auto. split_hyp.
+    eapply DSig_regularity in H; auto.
+    destruct H as [k0 [jk0 [Ha HA]]].
+    exists (i + (k + k0)); split. lia.
     replace a_Type with (incr i a_Type); auto.
     replace G with (G ++ nil).
     eapply DTyping_weakening1; eauto.
     replace nil with (IncG i nil); auto.
-    apply DTyping_cumul with (j := i + j); auto.
     eapply DTyping_incr; auto.
+    apply DTyping_cumul with (j := k0); auto. lia.
     all: simpl_env; auto.
   - (* var *)
-    apply DTyping_cumul with (j := j); auto.
-    eapply DCtx_regularity in H0; eauto.
-  - eapply DT_Type; eauto. eapply DTyping_DCtx; eauto.
-  - apply DTyping_a_Arrow_inversion in IHDTyping1. split_hyp. eauto.
+    eapply DCtx_regularity in H; eauto.
+    destruct H as [k0 [j0k HA]].
+    exists (k + k0); split. lia.
+    apply DTyping_cumul with (j := k0); auto. lia.
+  - destruct IHDTyping1 as [k0 [kk0 IHDTyping1]].
+    apply DTyping_a_Arrow_inversion in IHDTyping1. split_hyp. eauto.
   - pick fresh x.
+    destruct IHDTyping1 as [k [jk IHDTyping1]].
     move: (@DTyping_a_Pi_inversion x _ _ _ _ _ _ IHDTyping1 ltac:(auto)) => h0.
     destruct h0; split_hyp.
     + rewrite (subst_tm_intro x). auto.
       replace (a_Type) with (subst_tm a x a_Type).
+      exists k; split; auto.
       eapply DTyping_subst1; eauto. simpl; auto.
 Qed.
 
 (* Just convenient to have... *)
-Corollary DTyping_regularity_a_Pi : forall L S G b A j B k,
-  (forall x, x `notin` L -> DTyping S (x ~ Tm A j ++ G) (b ^ x) (B ^ x) k) ->
-  (forall x, x `notin` L -> DTyping S (x ~ Tm A j ++ G) (B ^ x) a_Type k).
+Corollary DTyping_regularity_a_Pi : forall L S G b A i B j,
+  (forall x, x `notin` L -> DTyping S (x ~ Tm A i ++ G) (b ^ x) (B ^ x) j) ->
+  exists k, (forall x, x `notin` L \u dom G \u dom S -> DTyping S (x ~ Tm A i ++ G) (B ^ x) a_Type k).
 Proof.
   intros.
-  specialize (H x H0).
-  apply (DTyping_regularity H).
-Qed.
-
-Lemma PiLT : forall S G b A j B k, DTyping S G b (a_Pi A j B) k -> j < k.
-intros.
-move: (DTyping_regularity H) => h0.
-pick fresh y.
-eapply DTyping_a_Pi_inversion in h0. split_hyp. auto. eauto.
+  pick fresh x; spec x.
+  apply DTyping_regularity in H as [k [jk TB]].
+  exists k.
+  move => y yL.
+  eapply DTyping_rename1; eauto.
 Qed.
 
 Lemma DTyping_a_Abs_inversion :
   forall x S G b B k, DTyping S G (a_Abs b) B k ->
        x `notin` dom G \u dom S ->
-       exists j1 j2 A1 A2,
-       DTyping S (x ~ Tm A1 j1 ++ G) (b ^ x) A2 j2 /\
-         ((DEquiv S B (a_Arrow A1 A2) /\ j1 = j2 /\ j2 <= k) \/
-         (exists A3, (DEquiv S B (a_Pi A1 j1 A3)) /\ A2 = (A3 ^ x)
-                     /\ j1 < j2 /\ j1 < k /\ j2 <= k
-                     /\ x `notin` fv_tm A3)).
+       exists i A1 A2,
+       DTyping S (x ~ Tm A1 i ++ G) (b ^ x) A2 k /\
+         (exists A3, (DEquiv S B (a_Pi A1 i A3)) /\ A2 = (A3 ^ x)
+                     /\ x `notin` fv_tm A3).
 Proof.
   intros.
   dependent induction H.
-  + exists k. exists k. exists A. exists B.
+  + (* arrow *) admit.
+    (* exists k. exists k. exists A. exists B.
     split.
     pick fresh y. spec y.
     eapply DTyping_rename1; eauto.
-    left. split; eauto with lc.
-  + exists j. exists k. exists A. exists (B ^ x).
+    left. split; eauto with lc. *)
+  + exists i. exists A. exists (B ^ x).
     pick fresh y. spec y.
     split.
     eapply DTyping_rename2; eauto.
-    right.
     exists B. split; auto with lc.
     eapply DE_Refl; eauto.
     eapply (lc_a_Pi_exists y); eauto with lc.
     repeat split; eauto.
     move: DTyping_fv => [_ [_ h]].
     move: (h _ _ _ _ _ H0) => [f1 f2].
-    simpl in f2.
-    rewrite <- fv_tm_open_tm_wrt_tm_lower in f2. fsetdec.
-  + edestruct IHDTyping1 as [j0 [j2 [A2 [A3 h]]]]. eauto. auto.
-    split_hyp.
-    have DC: DCtx S (x ~ Tm A2 j0 ++ G). eauto with ctx.
-    inversion DC. subst.
-    destruct H4.
-    ++ exists j0. exists j2. exists A2. exists A3.
-       split_hyp. subst.
-       split. eapply DT_Conv; eauto.
-       eapply DT_Conv; eauto.
-       eapply DTyping_regularity; eauto.
-       eapply DE_Refl; eauto with lc.
-       left. split. eapply DE_Trans; eauto. lia.
-    ++ move: H4 => [A4 h].  split_hyp. subst.
-       exists j0. exists j2. exists A2. exists (A4 ^ x).
-       split.
-       auto.
-       right.
-       exists A4.
-       repeat split.
-       eapply DE_Trans. eapply DE_Sym. eauto. eauto.
-       all: try lia.
-    move: DTyping_fv => [_ [_ h]].
-    move: (h _ _ _ _ _ H3) => [f1 f2].
-    simpl in f2.
-    rewrite <- fv_tm_open_tm_wrt_tm_lower in f2. fsetdec.
+    rewrite <- fv_tm_open_tm_wrt_tm_lower in f1.
+    simpl in f1.
+    have fxy : x `notin` singleton y by clear H6 h f1 f2; fsetdec.
+    clear Fr h f2. fsetdec.
+  + edestruct IHDTyping1 as [j0 [A2 [A3 [H4 [A4 [H5 [H6 H7]]]]]]]; eauto.
+    subst.
+    exists j0. exists A2. exists (A4 ^ x).
+    split; eauto.
+    exists A4.
+    split; eauto.
 Unshelve.
 all: exact nil.
-Qed.
+Admitted.
 
 Lemma DTyping_a_App_inversion :
   forall S G b0 b1 B k, DTyping S G (a_App b0 b1) B k ->
-    (exists A, DTyping S G b0 (a_Arrow A B) k /\ DTyping S G b1 A k) \/
     (exists j A B0, DTyping S G b0 (a_Pi A j B0) k /\ DTyping S G b1 A j
                     /\ DEquiv S B (open B0 b1)).
 Proof.
   intros.
   dependent induction H.
-  + left. clear IHDTyping1 IHDTyping2.
-    eexists. eauto.
-  + right. repeat eexists. eauto. eauto.
-    eapply DE_Refl.
-    have LC: lc_tm (a_Pi A j B). eauto with lc.
-    inversion LC.
-    pick fresh x.
-    rewrite (subst_tm_intro x); auto.
-    eapply subst_tm_lc_tm; eauto with lc.
+  + (* arrow *) admit.
+  + exists i. exists A. exists B.
+    repeat split; eauto with lc.
   + edestruct IHDTyping1; eauto.
-    ++ left. move: H2 => [A0 [TA1 TA2]].
-       move: (DTyping_regularity TA1) => h.
-       apply DTyping_a_Arrow_inversion in h. split_hyp.
-       eexists. split.
-       eapply DT_Conv. eauto.
-       2: { eapply DE_Arrow. eapply DE_Refl. eauto with lc. auto. }
-       eapply DT_Arrow; eauto. auto.
-    ++ right. move: H2 => [i [A0 [B0 T]]]. split_hyp. subst.
-       move: (DTyping_regularity H2) => h.
-       pick fresh x.
-       eapply DTyping_a_Pi_inversion in h; eauto. split_hyp.
-       eexists. eexists. eexists.
-       repeat split; eauto.
-Unshelve.
-all: exact nil.
-Qed.
+    move: H3 => [A0 [B0 T]]. split_hyp. subst.
+    move: (DTyping_regularity H3) => [k0 [xk TPi]].
+    pick fresh y.
+    eapply DTyping_a_Pi_inversion in TPi; eauto. split_hyp.
+    eexists. eexists. eexists.
+    repeat split; eauto.
+Admitted.
 
 Lemma DTyping_a_Const_inversion :
   forall S G x i B k,
@@ -224,7 +190,7 @@ Proof.
     repeat split; eauto with lc. lia.
   + edestruct IHDTyping1; eauto.
     rename x0 into a0.
-    move: H2 => [A0 [j0 h]]. split_hyp.
+    move: H3 => [A0 [j0 h]]. split_hyp.
     exists a0. exists A0. exists j0.
     repeat split; eauto with lc.
 Qed.
